adjust insert and make_array_naive to use the output of the script I'm working on

tmonad/make_array_naive.v
@@ -6,42 +6,99 @@ Require Import Braun.logical.sequence.
 Require Import Braun.common.braun.
 Require Import Braun.common.array.
 Require Import Braun.common.util.
-Require Import Braun.common.log.
+Require Import Braun.common.log Braun.common.le_util.
+Require Import Arith Arith.Even Arith.Div2 Omega.
 
 Section make_array_naive.
   Variable A : Set.
+
+  Fixpoint man_time' n : nat :=
+    match n with
+      | 0 => 1
+      | S n' => man_time' n' + 3 * (fl_log n') + 5
+    end.
 
   Program Fixpoint make_array_naive xs : 
     {! b !:! @bin_tree A
        !<! c !>!
        let n := length xs in
        Braun b n
-       /\ c = man_time n
+       /\ c = man_time' n
        /\ SequenceR b xs !} :=
-    match xs with
-      | nil      => 
-        <== bt_mt
-      | (cons x xs') => 
-        bt  <- make_array_naive xs';
-        bt' <- insert x bt;
-        <== bt'  
-    end.
+(match xs with
+   | nil => 
+     (++;
+      (<== bt_mt))
+   | cons x xs' => 
+     (anorm5 <- (make_array_naive xs');
+      (anorm6 <- (insert x anorm5);
+       (++; ++; ++;
+        (<== anorm6))))
+ end).
 
+  Obligation Tactic := auto.
   Next Obligation.
   Proof.
-    rename H into IH.
-    clear H3.
-    rename H0 into B.
-    rename H2 into SR.
-    remember (IH (length xs') B) as IND.
-    destruct IND as [BT [SEQ XN]].
+    intros xs x xs' Heqxs; subst xs.
+    intros bt.
+    intros [n [Bb [Heqn Sb]]].
+    subst n.
+    intros bt'.
+    intros junk; clear junk.
+    intros xn IH. 
+    intros xn0.
+    intros [Bbt [Heqxn0 Sbt]].
+    subst xn0.
+    intros n; subst n.
+
+    remember (IH (length xs') Bb) as CONJ.
+    clear HeqCONJ.
+    destruct CONJ as [Bbt' [SR_IND Heqxn]].
+
     repeat constructor; auto.
-    
-    assert (xn = cl_log (S (length xs'))); [| omega].
-    remember (IH (length xs') B).
-    subst.
-    assert (fl_log (length xs') + 1 = S (fl_log (length xs'))) as EQ; [omega | ].
-    rewrite EQ.
-    apply fl_log_cl_log_relationship.
+
+    subst xn.
+    simpl.
+    omega.
   Qed.
+
+
+  (* TODO: simplify this to something like:
+      man_time' n <= 8 * n * fl_log n + 1
+   *)
+
+  Lemma man_time'_nlogn:
+    forall n,
+      man_time' n <= n * (3 * fl_log n + 5) + 1.
+  Proof.
+    induction n as [|n].
+    simpl; omega.
+
+    unfold man_time'; fold man_time'.
+
+    apply (le_trans (man_time' n + 3 * fl_log n + 5)
+                    (( n * (3 * fl_log n + 5) + 1) + 3 * fl_log n + 5)
+                    (S n * (3 * fl_log (S n) + 5) + 1)).
+    repeat (apply le_plus_left).
+    assumption.
+
+    replace (S n * (3 * fl_log (S n) + 5))
+    with (n * (3 * fl_log (S n) + 5) + (3 * fl_log (S n) + 5)).
+    
+    assert (n * (3 * fl_log n + 5) <= n * (3 * fl_log (S n) + 5)).
+    apply le_mult_right.
+    apply le_plus_left.
+    apply le_mult_right.
+    apply fl_log_monotone.
+
+    assert (3 * fl_log n + 5 <= 3 * fl_log (S n) + 5).
+    apply le_plus_left.
+    apply le_mult_right.
+    apply fl_log_monotone.
+    omega.
+    
+    unfold mult; fold mult; omega.
+Qed.
+
+
 End make_array_naive.
